---
title: "Lag polynomials"
format: html
---

A $p$-th degree lag polynomial is given by:

$$
\alpha(L) = \alpha_0 + \alpha_1L + \cdots + \alpha_pL^p,
$$
where $L$ is the lag operator, defined by the relation $L^jx_t=x_{t-j}.$

We define a filter given by $\alpha(L)$ to an input process $\{x_t\}$, we get a weighted average of the current and $p$ most recent values of the process:

$$
\begin{aligned}
\alpha(L)x_t &= \alpha_0x_t + \alpha_1Lx_t + \alpha_2L^2x_t + \cdots + \alpha_pL^px_t \\
&= \alpha_0x_t + \alpha_1x_{t-1}+ \alpha_2x_{t-2} + \cdots + \alpha_px_{t-p} \\
&= \sum_{j=0}^p \alpha_jx_{t-j}
\end{aligned}
$$


## Product of Filters

Let $\{\alpha_j\}$ and $\{\beta_j\}$ be two arbitrary sequences of real numbers and define the sequence $\{\delta_j\}$ by the relation

$$
\begin{gathered}
\delta_0 = \alpha_0\beta_0, \\
\delta_1 = \alpha_0\beta_1 + \alpha_1\beta_0, \\
\delta_2 = \alpha_0\beta_2 + \alpha_1\beta_1 + \alpha_2\beta_0, \\
\vdots \\
\delta_j = \alpha_0\beta_j + \alpha_1\beta_{j-1} + \alpha_2\beta_{j-2} + \cdots + \alpha_{j-1}\beta_{1} + \alpha_{j}\beta_{0}, \\
\vdots \\
\end{gathered}
$$ {#eq-convolution}


The sequence $\{\delta_j\}$ created from this convuluted formula is called the convolution of $\{\alpha_j\}$ and $\{\beta_j\}.$

For example, for $\alpha(L)=1+\alpha_1L$ and $\beta(L)=1+\beta_1L$, we have

$$
\delta(L)=(1+\alpha_1L)(1+\beta_1L) = 1+ (\alpha_1+\beta_1)L + \alpha_1\beta_1L^2.
$$

Filters are commutative:

$$
\alpha(L)\beta(L) = \beta(L)\alpha(L)
$$

## Inverses

The inverse of $\alpha(L)$ is denoted as $\alpha(L)^{-1}$ or $1/\alpha(L)$:

$$
\alpha(L)\alpha(L)^{-1}=1
$$
Define a $p$-th degree lag polynomial $\phi(L)$

$$
\phi(L) = 1-\phi_1L-\phi_2L^2-\cdots-\phi_pL^p.
$$ {#eq-lag-ploy}

@eq-lag-ploy is often used to construct AR processes.

Now let's calculate its inverse, $\psi(L) = \phi(L)^{-1}.$

$$
\psi(L) = \psi_0 + \psi_1L + \psi_2L^2 + \cdots 
$$

By the convolution formula ([-@eq-convolution]), we have

$$
\begin{aligned}
\text{constant}:&\quad  \psi_0 =1 \\
L: &\quad  \psi_1-\psi_0\phi_1 = 0 \Longrightarrow \psi_1 = \phi_1 \\
L^2: &\quad  \psi_2-\psi_1\phi_1-\psi_0\phi_2 = 0 \Longrightarrow \psi_2 = \phi_1^2 + \phi_2 \\
\vdots \\
L^p: &\quad  \psi_p - \psi_{p-1}\phi_1 - \psi_{p-2}\phi_2 - \cdots - \psi_{1}\phi_{p-1} - \psi_{0}\phi_p = 0 \\
L^{p+1}: &\quad  \psi_{p+1} - \psi_{p}\phi_1 - \psi_{p-1}\phi_2 - \cdots - \psi_{2}\phi_{p-1} - \psi_{1}\phi_p = 0 \\
\vdots
\end{aligned}
$$

::: {#exm-inverse}
Consider a 1st degree lag polynomial $\phi(L)=1-\phi L$, its inverse $\psi(L)$ can be calculated as 

$$
\begin{aligned}
\text{constant}: &\quad \psi_0 =1  \\
L: &\quad \psi_1 - \psi_0\phi = 0 \Longrightarrow \psi_1 = \phi \\
L^2: &\quad \psi_2 - \psi_1\phi = 0 \Longrightarrow \psi_2 = \phi^2 \\
L^3: &\quad \psi_3 - \psi_2\phi = 0 \Longrightarrow \psi_3 = \phi^4 \\
\vdots 
\end{aligned}
$$
$\psi(L) = 1 + \phi L + \phi^2 L^2 + \phi^3 L^3 + \cdots.$
:::





## Stability Condition



The solution sequence $\{\psi_j\}$ eventually starts declining at a geometric rate if the **stability condition** holds. The condition states:

All the roots of the $p$-th degree polynomial equation in $z$

$$
\phi(z) = 0 \text{ where } \phi(z) \equiv 1-\phi_1z-\phi_2z^2-\cdots-\phi_pz^p
$$
are greater than 1 in absolute value (lie *outside* the unit circle).


Equivalently, we can consider the roots of the reciprocal polynomial defined as (basically this means inverting the order of the coefficients)

$$
\phi^*(z) = z^p\phi(z^{-1}) = z^p - \phi_1z^{p-1} - \dots - \phi_p.
$$
The stability condition can be stated as:

All the roots of 

$$
\phi^*(z) \equiv z^p - \phi_1z^{p-1} - \dots - \phi_p =0
$$
are less than 1 in the absolute value (i.e., lie *inside* the unit circle).





































